secure_api/box/functor_box/Box.PKAE.fsti
@@ -22,71 +22,76 @@ module Plain = Box.Plain
 module ID = Box.Index
 
 
-val nonce: t:Type0{hasEq t}
-val cipher: Type0
-val sub_id: t:Type0{hasEq t}
-val key_id: Type0
-
-val compose_ids: s1:sub_id -> s2:sub_id{s2 <> s1} -> key_id
+val nonce': t:Type0{hasEq t}
+val cipher': Type0
+val sub_id': t:Type0{hasEq t}
+val key_id': Type0
+val plain': Type0
 
 val valid_plain_length: nat -> bool
 val valid_cipher_length: nat -> bool
-val plain_t: Type0
-val length: p:plain_t -> n:nat{valid_plain_length n}
 
-
-type index_module = im:ID.index_module{ID.id im == sub_id}
-type plain_index_module = im:ID.index_module{ID.id im == key_id}
+type index_module = im:ID.index_module{ID.id im == sub_id'}
+type plain_index_module = im:ID.index_module{ID.id im == key_id'}
 type plain_module = Plain.plain_module
-//let id (im:index_module) = ID.id im
-//let kid (im:key_index_module) = ID.id im
 
-type log_region (im:plain_index_module) =
-  r:MR.rid{disjoint r (ID.get_rgn im)}
+type log_region (pim:plain_index_module) =
+  r:MR.rid{disjoint r (ID.get_rgn pim)}
 
-type message_log_key (im:plain_index_module) = (nonce*(i:ID.id im))
-type message_log_value (im:plain_index_module) (i:ID.id im) = (cipher*Plain.protected_plain_t im plain_t i)
+val aux_t: skey:Type0 -> pkey:Type0 -> (im:index_module) -> (pim:plain_index_module) -> (pm:plain_module) -> rgn:log_region pim -> Type u#1
+
+abstract noeq type pkae_module =
+  | PKAE:
+    nonce: (t:Type0{t == nonce'}) ->
+    cipher: (t:Type0{t == cipher'}) ->
+    sub_id: (t:Type0{t == sub_id'}) ->
+    key_id: (t:Type0{t == key_id'}) ->
+    plain: (t:Type0{t == plain'}) ->
+    skey: (t:Type0) ->
+    pkey: (t:Type0) ->
+    pkey_from_skey: (sk:skey -> pk:pkey) ->
+    compatible_keys: (sk:skey -> pk:pkey -> t:Type0{t <==> pk =!= pkey_from_skey sk}) ->
+    im:ID.index_module{ID.id im == sub_id} ->
+    pim:ID.index_module{ID.id pim == key_id} ->
+    pm:Plain.plain_module{Plain.get_plain pm == plain /\ Plain.valid_length #pm == valid_plain_length} ->
+    rgn:log_region pim ->
+    enc: (plain -> n:nonce -> pk:pkey -> sk:skey{compatible_keys sk pk} -> GTot cipher) ->
+    dec: (c:cipher -> n:nonce -> pk:pkey -> sk:skey -> GTot (option plain)) ->
+    aux: (aux_t skey pkey im pim pm rgn) ->
+    pkae_module
+
+
+
+val compose_ids: pkae:pkae_module ->  s1:pkae.sub_id -> s2:pkae.sub_id{s2 <> s1} -> pkae.key_id
+
+val length: pkae:pkae_module -> p:pkae.plain -> n:nat{valid_plain_length n}
+
+
+
+type message_log_key (im:plain_index_module) = (nonce'*(i:ID.id im))
+type message_log_value (im:plain_index_module) (i:ID.id im) = (cipher'*Plain.protected_plain_t im plain' i)
 type message_log_range (im:plain_index_module) (k:message_log_key im) = (v:message_log_value im (snd k))
 type message_log_inv (im:plain_index_module) (f:MM.map' (message_log_key im) (message_log_range im)) = True //t:Type0{t = True}
 type message_log (im:plain_index_module) (rgn:log_region im) =
   MM.t rgn (message_log_key im) (message_log_range im) (message_log_inv im)
 
-val pkey: Type0
-val skey: Type0
-
-val pkey_from_skey: sk:skey -> pk:pkey
-
-val compatible_keys: sk:skey -> pk:pkey -> t:Type0{t <==> pk =!= pkey_from_skey sk}
-
-val aux_t: (im:index_module) -> (pim:plain_index_module) -> (pm:plain_module{Plain.get_plain pm == plain_t}) -> rgn:log_region pim -> Type u#1
-
-abstract noeq type pkae_module =
-  | PKAE:
-    im:index_module{ID.id im == sub_id} ->
-    pim:plain_index_module ->
-    pm:Plain.plain_module{Plain.get_plain pm == plain_t /\ Plain.valid_length #pm == valid_plain_length} ->
-    rgn:log_region pim ->
-    enc: (plain_t -> n:nonce -> pk:pkey -> sk:skey{compatible_keys sk pk} -> GTot cipher) ->
-    dec: (c:cipher -> n:nonce -> pk:pkey -> sk:skey -> GTot (option plain_t)) ->
-    aux: (aux_t im pim pm rgn) ->
-    pkae_module
 
 val get_message_log_region: pkm:pkae_module -> Tot (log_region pkm.pim)
 val get_message_logGT: pkm:pkae_module -> Tot (message_log pkm.pim (get_message_log_region pkm)) //TODO: MK: would prefer this to be GTot
 
 val create: rgn:(r:MR.rid{extends r root /\ is_eternal_region r /\ is_below r root}) -> St (pkae_module)
 
-val zero_bytes: (n:nat{valid_plain_length n}) -> plain_t //b:bytes{Seq.length b = n /\ b=Seq.create n (UInt8.uint_to_t 0)}
+val zero_bytes: (n:nat{valid_plain_length n}) -> plain' //b:bytes{Seq.length b = n /\ b=Seq.create n (UInt8.uint_to_t 0)}
 //TODO: MK this can be modelled better
 
-val pkey_to_subId: #pkm:pkae_module -> pk:pkey -> ID.id pkm.im
-val pkey_to_subId_inj: #pkm:pkae_module -> pk:pkey -> Lemma
+val pkey_to_subId: #pkm:pkae_module -> pk:pkm.pkey -> ID.id pkm.im
+val pkey_to_subId_inj: #pkm:pkae_module -> pk:pkm.pkey -> Lemma
   (requires True)
   (ensures (forall pk' . pkey_to_subId #pkm pk == pkey_to_subId #pkm pk' <==> pk == pk'))
   [SMTPat (pkey_to_subId #pkm pk)]
 
 #set-options "--z3rlimit 2000 --max_ifuel 1 --max_fuel 0"
-val nonce_is_fresh: (pkm:pkae_module) -> (i:ID.id pkm.pim) -> (n:nonce) -> (h:mem) ->
+val nonce_is_fresh: (pkm:pkae_module) -> (i:ID.id pkm.pim) -> (n:nonce') -> (h:mem) ->
   (t:Type0{t <==>
     (MR.m_contains #(get_message_log_region pkm) (get_message_logGT pkm) h
       /\ MM.fresh #(get_message_log_region pkm)(get_message_logGT pkm) (n,i) h)})
@@ -98,7 +103,7 @@ val nonce_is_fresh: (pkm:pkae_module) -> (i:ID.id pkm.pim) -> (n:nonce) -> (h:me
 
 val invariant: pkae_module -> mem -> Type0
 
-val gen: unit -> ST (keypair:(pkey*skey){fst keypair == pkey_from_skey (snd keypair)})
+val gen: pkm:pkae_module -> ST (keypair:(pkm.pkey*pkm.skey){fst keypair == pkm.pkey_from_skey (snd keypair)})
   (requires (fun h0 -> True))
   (ensures (fun h0 _ h1 ->
     modifies_none h0 h1
@@ -109,24 +114,24 @@ let honest pkm i = ID.honest pkm.pim i
 let dishonest pkm i = ID.dishonest pkm.pim i
 
 val encrypt: pkm:pkae_module ->
-             n:nonce ->
-             sk:skey ->
-             pk:pkey{compatible_keys sk pk} ->
-             m:(Plain.protected_plain_t pkm.pim (Plain.get_plain pkm.pm) (compose_ids (pkey_to_subId #pkm pk) (pkey_to_subId #pkm (pkey_from_skey sk)))) ->
-             ST cipher
+             n:pkm.nonce ->
+             sk:pkm.skey ->
+             pk:pkm.pkey{pkm.compatible_keys sk pk} ->
+             m:(Plain.protected_plain_t pkm.pim (Plain.get_plain pkm.pm) (compose_ids pkm (pkey_to_subId #pkm pk) (pkey_to_subId #pkm (pkm.pkey_from_skey sk)))) ->
+             ST pkm.cipher
   (requires (fun h0 ->
-    let i = compose_ids (pkey_to_subId #pkm pk) (pkey_to_subId #pkm (pkey_from_skey sk)) in
+    let i = compose_ids pkm (pkey_to_subId #pkm pk) (pkey_to_subId #pkm (pkm.pkey_from_skey sk)) in
     registered pkm i
     /\ nonce_is_fresh pkm i n h0
     /\ invariant pkm h0
   ))
   (ensures  (fun h0 c h1 ->
-    let i = compose_ids (pkey_to_subId #pkm pk) (pkey_to_subId #pkm (pkey_from_skey sk)) in
+    let i = compose_ids pkm (pkey_to_subId #pkm pk) (pkey_to_subId #pkm (pkm.pkey_from_skey sk)) in
     modifies (Set.singleton pkm.rgn) h0 h1 // stateful changes even if the id is dishonest.
     /\ ((honest pkm i /\ b2t pkae) // Ideal behaviour if the id is honest and the assumption holds
-               ==> eq2 #cipher c (pkm.enc (zero_bytes (Plain.length #pkm.pim #pkm.pm #i m)) n pk sk))
+               ==> eq2 #pkm.cipher c (pkm.enc (zero_bytes (Plain.length #pkm.pim #pkm.pm #i m)) n pk sk))
     /\ ((dishonest pkm i \/ ~(b2t pkae)) // Concrete behaviour otherwise.
-                  ==> eq2 #cipher c (pkm.enc (Plain.repr #pkm.pim #pkm.pm #i m) n pk sk))
+                  ==> eq2 #pkm.cipher c (pkm.enc (Plain.repr #pkm.pim #pkm.pm #i m) n pk sk))
     // The message is added to the log. This also guarantees nonce-uniqueness.
     /\ MR.m_contains #(get_message_log_region pkm)(get_message_logGT pkm) h1
     /\ MR.witnessed (MM.contains #(get_message_log_region pkm) (get_message_logGT pkm) (n,i) (c,m))
@@ -135,18 +140,18 @@ val encrypt: pkm:pkae_module ->
   ))
 
 val decrypt: pkm:pkae_module ->
-             n:nonce ->
-             sk:skey ->
-             pk:pkey{compatible_keys sk pk} ->
-             c:cipher ->
-             ST (option (Plain.protected_plain_t pkm.pim (Plain.get_plain pkm.pm) (compose_ids (pkey_to_subId #pkm pk) (pkey_to_subId #pkm (pkey_from_skey sk)))))
+             n:pkm.nonce ->
+             sk:pkm.skey ->
+             pk:pkm.pkey{pkm.compatible_keys sk pk} ->
+             c:pkm.cipher ->
+             ST (option (Plain.protected_plain_t pkm.pim (Plain.get_plain pkm.pm) (compose_ids pkm (pkey_to_subId #pkm pk) (pkey_to_subId #pkm (pkm.pkey_from_skey sk)))))
   (requires (fun h0 ->
-    let i = compose_ids (pkey_to_subId #pkm pk) (pkey_to_subId #pkm (pkey_from_skey sk)) in
+    let i = compose_ids pkm (pkey_to_subId #pkm pk) (pkey_to_subId #pkm (pkm.pkey_from_skey sk)) in
     registered pkm i
     /\ invariant pkm h0
   ))
   (ensures  (fun h0 p h1 ->
-    let i = compose_ids (pkey_to_subId #pkm pk) (pkey_to_subId #pkm (pkey_from_skey sk)) in
+    let i = compose_ids pkm (pkey_to_subId #pkm pk) (pkey_to_subId #pkm (pkm.pkey_from_skey sk)) in
     h0 == h1
     /\ invariant pkm h1
     /\ ((~(b2t pkae_int_ctxt) \/ dishonest pkm i) ==> // Concrete behaviour of the id is dishonest or if the assumption doesn't hold.
